small fix

code/rocq/elpi.v
@@ -1,21 +1,21 @@
 From mathcomp Require Import all_ssreflect.
-From det Require Import lang.
+From det Require Import lang run_prop.
 
 Import Language.
 
 Module Nur (U : Unif).
 
-  Module Run := Run(U).
-  Import Run U Language.
+  Module RunP := RunP(U).
+  Import RunP Run U Language.
 
   Inductive G := 
     | call : Tm -> G
     | cut : list (list G) -> G.
   Definition alt := (list G).
 
-  Definition next_alt {T:Type} a (k : list G -> list alt -> option  T) :=
+  (* Definition next_alt {T:Type} a (k : list G -> list alt -> option  T) :=
     if a is [:: gl & a] then k gl a
-    else None.
+    else None. *)
 
   Definition save_alt_ca (a : A) alts :=
     match a with
@@ -34,7 +34,8 @@ Module Nur (U : Unif).
     F p t s = [:: b & bs ] -> 
       nur (save_alt a b gl) (more_alt a bs gl) r -> 
         nur [::call t & gl] a r
-  | FailE a g al r : nur a al r -> nur g (a :: al) r.
+  | FailE p t s gl a al r : 
+    F p t s = [::] -> nur a al r -> nur [::call t & gl] (a :: al) r.
 
   Definition nur' p a r :=
     match a with
@@ -50,8 +51,12 @@ Module Nur (U : Unif).
   Definition add_cas lA lB : alt :=
     [seq add_ca gl lB | gl <- lA].
 
-  Definition add_alt lA lB : list alt :=
-    flatten [seq [seq la ++ lb | lb <- lB] | la <- lA].
+  Definition add_alt (lB0 lA lB:list (alt)) : list  alt :=
+    match lA with
+    | [::] => [::]
+    | x :: xs =>
+      ([seq x ++ y | y <- lB] : list alt) ++ flatten [seq [seq la ++ lb | lb <- lB0] | la <- xs]
+    end.
 
   Fixpoint state_to_list (A: state) (bt : list alt) : list alt :=
     match A with
@@ -63,22 +68,34 @@ Module Nur (U : Unif).
       let lB := state_to_list B bt in
       let lA := state_to_list A (lB ++ bt) in
       [seq add_cas la bt | la <- lA] ++ lB
-    | And A _ B => 
+    | And A B0 B => 
       let lA := state_to_list A bt in
       let lB := state_to_list B bt in
-      add_alt lA lB 
+      let lB0 := state_to_list B0 bt in
+      add_alt lB0 lA lB 
     end.
 
-  Goal forall p b0 x y z w s1 s2, 
+    (* 
+      ((x /\ b) \/ y ) /\a (z \/ w)
+
+      x /\ (z \/ w) \/ (y /\ a) =
+      x /\ z \/ x /\ w \/ y /\ a
+    *)
+
+  Goal forall p x y z w s1 s2 a, 
+    let f x := (Goal p (Call x)) in
     state_to_list (
       And 
-        (Or (Goal p (Call x)) s1 (Goal p (Call y))) b0 
-        (Or (Goal p (Call z)) s2 (Goal p (Call w)))) [::] = 
+        (Or (f x) s1 (f y)) (f a) 
+        (Or (f z) s2 (f w))) [::] = 
       [:: [:: call x; call z];
       [:: call x; call w];
-      [:: call y; call z];
-      [:: call y; call w]].
-  Proof. by []. Qed.
+      [:: call y; call a]].
+      (* [:: [:: call x]; [:: call z]; [:: call w]; 
+      [:: call y; call a]] *)
+  Proof.
+    move=>/=. by [].
+  Qed.
 
   Goal forall p a b s1 s2, 
     state_to_list (
@@ -96,32 +113,250 @@ Module Nur (U : Unif).
      [:: [:: call c; cut [:: [:: call b]]]; [:: call a]; [:: call b]].
   Proof. by []. Qed.
 
+  Definition same_state_next_alt l s r r1 :=
+    match next_alt s (get_state_run r) with 
+    | None => r1 = [::]
+    | Some (_,r) => state_to_list r l = r1
+    end.
+
   Definition runElpi A :=
-    forall s p r r1 b,
-      runb s A r b -> nur' p (state_to_list A [::]) r1 -> state_to_list (get_state_run r) [::] = r1.
+    forall s r b l,
+      runb s A r b -> forall p r1, nur' p (state_to_list A l) r1 -> 
+        same_state_next_alt l s r r1.
   
   Goal @runElpi OK.
   Proof.
-    rewrite/runElpi => s p r r1 b/=.
-    inversion 1; subst => //=.
-    - inversion 1; subst.
-      inversion H1; subst => //.
-      case: H8 => _ <-/=.
-
-
-  Lemma runExpandedb {s A s' B x xs}:
-     expandedb s A (Done s' B) b ->
-      state_to_list A [::] = x :: xs ->
-        nur p x xs r1 ->
-          state_to_list (get_state_run (Done s' B)) [::] = r1.
-
-  Lemma runElpi {s p A x xs r r1}:
-    state_to_list A [::] = x::xs ->
-    run s A r -> nur p x xs r1 -> state_to_list (get_state_run r) [::] = r1.
+    rewrite/runElpi.
+    inversion 1; subst => //=; inversion H1 => //; subst.
+    inversion 1.
+    by case: H7 => _ <-/=.
+  Qed.
+  
+  Goal @runElpi KO.
   Proof.
-    move=> + [b H].
-    elim: H p x xs r1; clear.
-    + move=> s s' A B b H p x xs r1. (* Qui Stop *)
+    rewrite/runElpi => s p r r1 b/=.
+    inversion 1; subst => //.
+  Qed.
+  
+  Goal @runElpi Top.
+  Proof.
+    rewrite/runElpi.
+    inversion 1; subst => //=.
+    - inversion H1; subst => //.
+      case: H2 => ??; subst.
+      inversion H3; subst => //.
+      case: H8 => ??; subst => /=.
+      by inversion 1.
+    - inversion H1; subst => //.
+      case: H3 => ??;subst.
+      inversion H4 => //.
+    - inversion H1; subst => //.
+      case: H4 => ??;subst.
+      inversion H5 => //.
+  Qed.
+
+  Lemma state_to_list_dead {A l}: state_to_list (dead A) l = [::].
+  Proof.
+    elim: A l => //.
+    + move=> A HA s B HB /= l.
+      by rewrite HB HA cats0/=.
+    + move=> A HA B0 _ B HB /= l.
+      by rewrite HA HB /add_alt/=.
+  Qed.
+
+  Lemma cats20 {T:Type} {A B : list (list T)} n: A ++ B = nseq n [::] -> 
+    exists n1 n2, n1 + n2 = n /\ A = nseq n1 [::] /\ B = nseq n2 [::].
+  Proof.
+    elim: n A B => //=.
+    + move=> []//[]// _; exists 0, 0 => //.
+    + move=> n H [|A0 As]//=.
+      + move=> B->.
+        exists 0, n.+1 => //.
+      + move=> B [->].
+        move=> /H[n1 [n2 [<- [->->]]]].
+        exists n1.+1, n2.
+        rewrite addSn//.
+  Qed.
+
+  Lemma cats20' {T:Type} {A B : list (list T)}: A ++ B = [::] -> A = [::] /\ B = [::].
+  Proof.
+    move=> /(cats20 0).
+    move=> [n1[n2[+[+ +]]]].
+    by case: n1 => //; case: n2 => //.
+  Qed.
+  
+  Lemma flatten_empty {T R : Type} {l: list T}:
+    @flatten R [seq [::] | _ <- l] = [::].
+  Proof. elim: l => //. Qed.
+
+  Lemma add_cas_compose {l1 l2 i}:
+    (add_cas^~ l1 \o add_cas^~ l2) i = add_cas i (l2 ++ l1).
+  Proof.
+    rewrite /add_cas/= -map_comp.
+    elim i => //=+ xs-> => -[]//=x.
+    by rewrite catA.
+  Qed.
+
+  Lemma expand_solve_state_to_list_cons1 {s1 A s2 A'}:
+     expand s1 A = Solved s2 A' -> forall r, exists l, state_to_list A r = [::] :: l.
+  Proof.
+    elim: A s1 s2 A' => //.
+    - by eexists.
+    - move=> p []//.
+    - move=> A HA s B HB s1 s2 C + r.
+      move=> /simpl_expand_or_solved[].
+        move=>[A'[HA'?]]; subst => /=.
+        have:= HA _ _ _ HA' ((state_to_list B r ++ r)).
+        by move=> [l]->/=; eexists.
+      move=> [B'[dA [HB' _]]]/=.
+      rewrite dA; rewrite state_to_list_dead/=.
+      by apply: HB HB' _.
+    - move=> A HA B0 _ B HB s1 s2 A1 + r.
+      move=> /simpl_expand_and_solved.
+      move=> [s3[A'[B'[HA' [HB' _]]]]]/=.
+      rewrite /add_alt.
+      have [l->]:= HA _ _ _ HA' r.
+      have [l'->]:= HB _ _ _ HB' r.
+      move=>/=.
+      by eexists.
+    Qed.
+  
+  Lemma next_alt_none_state_to_list {s B}:
+      failed B -> next_alt s B = None -> 
+        forall l, state_to_list B l = [::].
+  Proof.
+    elim: B => //.
+    - move=> A HA s1 B HB /= + + l.
+      case:ifP=>/eqP.
+        move=>->.
+        rewrite state_to_list_dead/=.
+        move=> fB.
+        case X: next_alt => [[]|]//.
+        rewrite HB//.
+      move=> dA fA.
+      case X: next_alt => [[s2 D]|]//.
+      rewrite HA//=.
+      case: ifP => /eqP.
+        by move=>->; rewrite state_to_list_dead.
+      move=> dB.
+      case: ifP => fB => //.
+      case Y: next_alt => [[]|]// _.
+      by apply: HB.
+    - move=> A HA B0 HB0 B HB/= + + l.
+      case: ifP=>/eqP.
+        move=>->.
+        by rewrite state_to_list_dead.
+      move=> dA/orP[].
+        move=>fA.
+        rewrite fA.
+        case X: next_alt => [[s3 C]|].
+          case: ifP => // fB0 _.
+          rewrite HB0///add_alt/=.
+          case Y: state_to_list => //[x xs].
+          rewrite flatten_empty cats0.
+
+          rewrite HA//.
+          admit.
+      rewrite HA//.
+    - move=> /andP[sA fB].  
+      rewrite success_failed//.
+      case X: next_alt => [[]|]//.
+      case Y: next_alt => [[s2 C]|]//.
+        case: ifP => // fB0.
+        admit.
+      by rewrite HB///add_alt/=flatten_empty.
+  Qed.
+
+      
+
+  (* Lemma next_alt_failed_state_to_list {s B s3 D}:
+    failed B ->  next_alt s B = Some (s3, D) -> 
+      forall l, state_to_list B l = state_to_list D l.
+  Proof.
+    elim: B s s3 D => //.
+    - move=> A HA s B HB s1 s2 C + + l.
+      move=> /=; case: ifP => /eqP .
+        move=>-> fB.
+        case X: next_alt => //[[s3 D]].
+        have ->:= HB _ _ _ fB X l.
+        move=>[_ <-]/=.
+        by rewrite state_to_list_dead/=.
+      move=> dA fA.
+      case X: next_alt => //[[s3 D]|].
+        move=> [_ <-]/=.
+        by rewrite (HA _ _ _ fA X).
+      case: ifP => /eqP dB//.
+      case: ifP => fB.
+        case Y: next_alt => //[[s3 D]][_ <-]/=.
+        rewrite state_to_list_dead/=(HB _ _ _ fB Y). *)
+
+
+  Goal forall s p, next_alt empty (Or OK s (Goal p Cut)) = Some (s, (Or Dead s (Goal p Cut))).
+  Proof. move=>//=. Qed.
+
+  Lemma expand_done:
+    forall p r1 x xs,
+      nur p x xs r1 ->
+    forall s A s1 B l,
+    expand s A = Solved s1 B ->
+        state_to_list A l = x :: xs ->
+          same_state_next_alt l s (Done s1 B) r1.
+  Proof.
+    move=> p r1 x xs H.
+    elim: H; clear => //.
+    + move=> + + A.
+      rewrite /same_state_next_alt/=.
+      {
+        elim: A => //.
+        + by move=> /= ?????[] _ <-[]<-/=.
+        + move=> p []//.
+        + { move=> A HA s B HB a s1 s2 C l.
+          move=> /simpl_expand_or_solved[].
+          - move=> [A' [HA'->]]/=.
+            clear HB.
+            have:= (success_dead1 (proj2 (expand_solved_success HA'))).
+            case: ifP => /eqP// dA' _.
+            remember (state_to_list B l ++ l) as r.
+            have [l']:= expand_solve_state_to_list_cons1 HA' r.
+            case Y: state_to_list => //=[y ys][??]; subst y l'.
+            have:= HA ys _ _ _ r HA' Y.
+            clear HA.
+            case X: next_alt=> //=[[s3 D]|]/=H[].
+              by rewrite -Heqr H.
+            subst ys.
+            move=>/=.
+            case: ifP => /eqP dB.
+              by rewrite dB state_to_list_dead.
+            move=><-.
+            clear a.
+            case: ifP => // fB/=.
+              case Z: next_alt => //[[s3 D]|]/=.
+                rewrite state_to_list_dead//=.
+                admit.
+              admit.
+            rewrite state_to_list_dead//.
+          - admit.
+        }
+        admit.
+      }
+    + all: admit.
+  Admitted.
+
+  Lemma runExpandedbDone {s s' A B b l}:
+    expandedb s A (Done s' B) b ->
+      forall (p0 : program) (r1 : seq alt),
+        nur' p0 (state_to_list A l) r1 -> same_state_next_alt l s (Done s' B) r1.
+  Proof.
+    remember (Done _ _) as d eqn:Hd => H.
+    elim: H s' B Hd => //; clear.
+    - move=> s s' A A' + s1 B [] ??; subst.
+      move: 
+
+  Lemma runElpiP: forall A, runElpi A.
+  Proof.
+    move=> A s r b H.
+    elim: H; clear.
+    + move=> s s' A B b H p r1. (* Qui Stop *)
       admit.
     + move=> s A B b H H1 p x xs r1. (* Qui Fail*)
       admit.
